src/Ingest/Ingest.v
@@ -13,178 +13,10 @@ Local Open Scope ZX_scope.
 
 (* Proving correctness of conversion *)
 
-Lemma swap_correct :
-  ZX_semantics ⨉ = swap.
-Proof. solve_matrix. Qed.
-
-(* A linear mapping which takes | x y1 ... yn > -> | y1 .. yn x > *)
-Fixpoint top_wire_to_bottom (n : nat) : Square (2 ^ n) :=
-  match n with
-  | 0   => I 1
-  | S k => match k with
-           | 0   => I 2
-           | S j => (@Mmult _ (2^n) _) ((I 2) ⊗ (top_wire_to_bottom k)) (swap ⊗ (j ⨂ (I 2)))
-           end
-  end.
-
-Open Scope matrix_scope.
-Definition bottom_wire_to_top (n : nat) : Square (2 ^ n) :=
-  (top_wire_to_bottom n)⊤.
-
-Lemma top_to_bottom_correct : forall n, ZX_semantics (top_to_bottom n) = top_wire_to_bottom n.
-Proof.
-  intros.
-  destruct n; [ reflexivity | ].
-  destruct n; [ easy | ].
-  induction n.
-  - easy.
-  - simpl.
-    simpl in IHn.
-    rewrite <- IHn.
-    rewrite n_wire_semantics.
-    rewrite kron_n_I.
-    rewrite 2 id_kron.
-    replace (2 * 2 ^ n)%nat with (2 ^ n * 2)%nat by lia.
-    easy.
-Qed.
-
-Lemma top_wire_to_bottom_ind : forall n, top_wire_to_bottom (S (S n)) = @Mmult _ (2 ^ (S (S n))) _ ((I 2) ⊗ top_wire_to_bottom (S n)) (swap ⊗ (I (2 ^ n))).
-Proof.
-  intros.
-  induction n.
-  - Msimpl.
-    simpl.
-    Msimpl.
-    easy.
-  - rewrite IHn.
-    simpl.
-    apply Mmult_simplify.
-    + apply kron_simplify; easy.
-    + apply kron_simplify; [easy | ].
-      rewrite kron_n_I.
-      rewrite id_kron.
-      replace (2 ^ n + (2 ^ n + 0))%nat with (2 ^ n * 2)%nat by lia.
-      easy.
-Qed.
-
-Lemma bottom_wire_to_top_ind : forall n, bottom_wire_to_top (S (S n)) = @Mmult _ (2 ^ (S (S n))) _ (swap ⊗ (I (2 ^ n))) ((I 2) ⊗ bottom_wire_to_top (S n)).
-Proof.
-  intros.
-  apply transpose_matrices.
-  unfold bottom_wire_to_top.
-  rewrite Mmult_transpose.
-  restore_dims.
-  rewrite Matrix.transpose_involutive.
-  restore_dims.
-  rewrite (kron_transpose 2 2 (2 ^ (S n)) (2 ^ S n)).
-  replace (Nat.pow 2 (S (S n)))%nat with ((2 * 2) * (2 ^ n))%nat by (simpl; lia).
-  rewrite (kron_transpose  (2 * 2) (2 * 2) (2 ^ n) (2 ^ n) swap (I (2 ^ n))).
-  rewrite 2 id_transpose_eq.
-  rewrite swap_transpose.
-  rewrite Matrix.transpose_involutive.
-  restore_dims.
-  rewrite (top_wire_to_bottom_ind n).
-  easy.
-Qed.
-
-(* Well foundedness of semantics *)
-
-Lemma WF_top_to_bottom (n : nat) : WF_Matrix (top_wire_to_bottom n).
-Proof.
-  destruct n; try auto with wf_db. 
-Qed.
-
-Global Hint Resolve WF_top_to_bottom : wf_db.
-
-Lemma WF_bottom_to_top (n : nat) : WF_Matrix (bottom_wire_to_top n).
-Proof. unfold bottom_wire_to_top. auto with wf_db. Qed.
-
-Global Hint Resolve WF_bottom_to_top : wf_db.
-
-Lemma bottom_to_top_correct : forall n, ZX_semantics (bottom_to_top n) = bottom_wire_to_top n.
-Proof.
-  intros.
-  unfold bottom_to_top.
-  unfold bottom_wire_to_top.
-  rewrite semantics_transpose_comm.
-  rewrite top_to_bottom_correct.
-  easy.
-Qed.
-
-Lemma swap_spec' : swap = ((ket 0 × bra 0)  ⊗ (ket 0 × bra 0) .+ (ket 0 × bra 1)  ⊗ (ket 1 × bra 0)
-  .+ (ket 1 × bra 0)  ⊗ (ket 0 × bra 1) .+ (ket 1 × bra 1)  ⊗ (ket 1 × bra 1)).
-Proof.
-  solve_matrix.
-Qed.
-
-Definition a_swap_semantics (n : nat) : Square (2 ^ n) :=
-  match n with
-  | 0   => I 1
-  | S k => (@Mmult _ (2 ^ n) _ ((I 2) ⊗ top_wire_to_bottom (k)) ((bottom_wire_to_top (S k))))
-  end.
-
-Lemma a_swap_correct : forall n, ZX_semantics (a_swap n) = a_swap_semantics n.
-Proof.
-  intros.
-  unfold a_swap_semantics.
-  destruct n; [ reflexivity | ].
-  rewrite <- bottom_to_top_correct.
-  rewrite <- top_to_bottom_correct.
-  simpl.
-  easy.
-Qed.
-
-Lemma WF_a_swap_semantics (n : nat) :
- WF_Matrix (a_swap_semantics n).
-Proof.
-  intros.
-  unfold a_swap_semantics.
-  destruct n; auto with wf_db.
-Qed.
-
-Global Hint Resolve WF_a_swap_semantics : wf_db.
-
-(* TODO: Move these to somewhere appropriate *)
-Lemma stack_semantics {n m o p} : forall (zx0 : ZX n m) (zx1 : ZX o p),
-  ZX_semantics (zx0 ↕ zx1) = ZX_semantics zx0 ⊗ ZX_semantics zx1.
-Proof. easy. Qed.
-
-(* TODO: Move these to somewhere appropriate *)
-Lemma compose_semantics {n m o} : forall (zx0 : ZX n m) (zx1 : ZX m o),
-  ZX_semantics (zx0 ⟷ zx1) = @Mmult (2 ^ n) (2 ^ m) (2 ^ o) (ZX_semantics zx1) (ZX_semantics zx0).
-Proof. easy. Qed.
-
-Lemma matrix_offset_swaps_comm_bottom_right :
-  I 2 ⊗ swap × (swap ⊗ I 2) = 
-  swap ⊗ I 2 × (I 2 ⊗ swap) × (swap ⊗ I 2) × (I 2 ⊗ swap).
-Proof.
-
-  (* solve_matrix. *)
-Admitted.
-
-(* Lemma matrix_offset_swaps_comm_top_left :
-  swap ⊗ I 2 × (I 2 ⊗ swap) = 
-  I 2 ⊗ swap × (swap ⊗ I 2) × (I 2 ⊗ swap) × (swap ⊗ I 2)
-Proof. solve_matrix. Qed. *)
-
-Lemma a_swap_ind : forall n, a_swap_semantics (S (S (S n))) = swap ⊗ (I (2 ^ (S n))) × (I 2 ⊗ a_swap_semantics (S (S n))) × (swap ⊗ (I (2 ^ (S n)))).
-Proof.
-  intros.
-  remember (swap ⊗ I (2 ^ S n) × (I 2 ⊗ a_swap_semantics (S (S n))) × (swap ⊗ I (2 ^ S n))) as right_side.
-  unfold a_swap_semantics.
-  rewrite bottom_wire_to_top_ind.
-  rewrite top_wire_to_bottom_ind.
-  rewrite <- Mmult_assoc.
-  rewrite kron_id_dist_l.
-  replace (2 ^ S n)%nat with (2 * 2 ^ n)%nat by (simpl; lia).
-  rewrite <- id_kron.
-Admitted.
-
-
 Lemma a_swap_sem_base : forall n, a_swap_semantics (S (S n)) = uc_eval (@SWAP (S (S n)) 0 (S n)).
 Proof.
   intros.
-  assert (forall q q', q = qubit0 \/ q = qubit1 -> q' = qubit0 \/ q' = qubit1 -> swap × (I 2 ⊗ (q × q'†)) × swap = (q × q'†) ⊗ I 2).
+  assert (forall q q', q = qubit0 \/ q = qubit1 -> q' = qubit0 \/ q' = qubit1 -> swap × (I 2 ⊗ (q × q'†%M)) × swap = (q × q'†%M) ⊗ I 2).
   {
     intros.
     destruct H; destruct H0; subst; solve_matrix.
@@ -195,8 +27,8 @@ Proof.
     unfold ueval_swap.
     simpl.
     gridify.
-    unfold bottom_wire_to_top.
-    unfold top_wire_to_bottom.
+    unfold Swaps.bottom_wire_to_top.
+    unfold Swaps.top_wire_to_bottom.
     rewrite unfold_pad.
     simpl.
     rewrite id_kron.
@@ -207,7 +39,7 @@ Proof.
     rewrite swap_transpose.
     Msimpl.
     apply swap_spec'.
-  - rewrite a_swap_ind.
+  - rewrite a_swap_semantics_ind.
     rewrite IHn.
     simpl.
     rewrite 2 denote_swap.
@@ -322,8 +154,10 @@ Qed.
 Lemma cnot_dim_conv : forall n m dim, (n <? m = true) -> (m <? dim = true) -> dim = (n + (m - n) + (dim - m))%nat.
 Proof.
   intros.
-  rewrite <- (le_plus_minus n m).
-  rewrite <- (le_plus_minus).
+  rewrite (Nat.add_comm n (m - n)).
+  rewrite (Nat.sub_add n m).
+  rewrite Nat.add_comm.
+  rewrite Nat.sub_add.
   easy.
   all: bdestruct (n <? m); try (exfalso; lia);
   bdestruct (m <? dim); try (exfalso; lia). 
@@ -702,7 +536,7 @@ Proof.
   rewrite pad_bot_top_semantics.
   repeat rewrite kron_assoc; try auto with wf_db; [| shelve].
   rewrite <- unpadded_cnot_simpl_args_sem.
-  rewrite <- minus_Sn_m; try lia.
+  rewrite Nat.sub_succ_l; try lia.
   destruct (m - n)%nat eqn:Hmn1; try (exfalso; lia).
   pose proof (unpadded_cnot_t_sem_equiv n0) as H_unpad_n0.
   rewrite <- H_unpad_n0.
@@ -752,7 +586,7 @@ Proof.
   rewrite pad_bot_top_semantics.
   repeat rewrite kron_assoc; try auto with wf_db; [| shelve].
   rewrite <- unpadded_cnot_simpl_args_sem.
-  rewrite <- minus_Sn_m; try lia.
+  rewrite Nat.sub_succ_l; try lia.
   destruct (n - m)%nat eqn:Hmn1; try (exfalso; lia).
   pose proof (unpadded_cnot_b_sem_equiv n0) as H_unpad_n0.
   rewrite <- H_unpad_n0.
