src/CoreData/CoreData.v
@@ -1,3 +1,4 @@
 Require Export ZXCore.
 Require Export Proportional.
 Require Export Swaps.
+Require Export StrongInduction.
