src/CoreData/StrongInduction.v
@@ -1,0 +1,60 @@
+(* Source: https://github.com/tchajed/strong-induction *)
+(* This should really be in the coq std library *)
+
+Local Open Scope nat_scope.
+(** Here we prove the principle of strong induction, induction on the natural
+numbers where the inductive hypothesis includes all smaller natural numbers. *)
+
+Require Import PeanoNat.
+
+Section StrongInduction.
+
+  Variable P:nat -> Prop.
+
+  (** The stronger inductive hypothesis given in strong induction. The standard
+  [nat ] induction principle provides only n = pred m, with [P 0] required
+  separately. *)
+  Hypothesis IH : forall m, (forall n, n < m -> P n) -> P m.
+
+(* @nocheck name *)
+  Lemma P0 : P 0.
+  Proof.
+    apply IH; intros.
+    exfalso; inversion H.
+  Qed.
+
+  Hint Resolve P0 : strong_ind_db.
+
+  Lemma pred_increasing : forall n m,
+      n <= m ->
+      Nat.pred n <= Nat.pred m.
+  Proof.
+    induction n; cbn; intros.
+    apply le_0_n.
+    induction H; subst; cbn; eauto.
+    destruct m; eauto.
+  Qed.
+
+  Hint Resolve le_S_n : strong_ind_db.
+
+  (** * Strengthen the induction hypothesis. *)
+
+  Local Lemma strong_induction_all : forall n,
+      (forall m, m <= n -> P m).
+  Proof.
+    induction n; intros;
+      match goal with
+      | [ H: _ <= _ |- _ ] =>
+        inversion H
+      end; eauto with strong_ind_db.
+  Qed.
+
+  Theorem strong_induction : forall n, P n.
+  Proof.
+    eauto using strong_induction_all.
+  Qed.
+
+End StrongInduction.
+
+Global Tactic Notation "strong" "induction" ident(n) := induction n using strong_induction.
+
