src/CoreRules/StackRules.v
@@ -4,6 +4,14 @@ Require Import SpiderInduction.
 
 Local Open Scope ZX_scope.
 
+Lemma stack_semantics {n m o p} : forall (zx0 : ZX n m) (zx1 : ZX o p),
+  ZX_semantics (zx0 ↕ zx1) = ZX_semantics zx0 ⊗ ZX_semantics zx1.
+Proof. easy. Qed.
+
+Lemma compose_semantics {n m o} : forall (zx0 : ZX n m) (zx1 : ZX m o),
+ZX_semantics (zx0 ⟷ zx1) = @Mmult (2 ^ n) (2 ^ m) (2 ^ o) (ZX_semantics zx1) (ZX_semantics zx0).
+Proof. easy. Qed.
+
 Lemma stack_assoc : 
 forall {n0 n1 n2 m0 m1 m2}
 	(zx0 : ZX n0 m0) (zx1 : ZX n1 m1) (zx2 : ZX n2 m2),
